another version

ICK2.v
@@ -1,3 +1,4 @@
+Set Implicit Arguments.
 Require Import Unicode.Utf8.
 Require Import Utf8_core.
 Require Import List.
@@ -15,12 +16,12 @@ Require Import Coq.Sets.Constructive_sets.
 Inductive apply_func (U1 U2:Type) (f:U1->U2) (S:Ensemble U1)
 : Ensemble U2 :=
 |In_apply_func: forall a:U1, In U1 S a->
-  In U2 (apply_func U1 U2 f S) (f a).
+  In U2 (apply_func f S) (f a).
 
 
 Lemma apply_func_rec : forall (U1 U2:Type) (f:U1->U2)
 (S:Ensemble U1) (a:U2),
-In U2 (apply_func U1 U2 f S) a ->
+In U2 (apply_func f S) a ->
 exists ia:U1, In U1 S ia /\ f ia=a.
 intros.
 inversion H.
@@ -35,7 +36,7 @@ Qed.
 *)
 Theorem apply_func_empty : forall (U1 U2:Type) (f:U1->U2)
 (S:Ensemble U1),
- (apply_func U1 U2 f (Empty_set U1)) = Empty_set U2.
+ (apply_func f (Empty_set U1)) = Empty_set U2.
 Proof.
 intros.
 apply Extensionality_Ensembles.
@@ -53,108 +54,117 @@ Qed.
 (***********************)
 
 (*
-  Notice the added (E t) term.
+  Notice the added (E t) Term.
 *)
-Inductive term : Set :=
-  | bottom : term
-  | var : nat → term
-  | e : term → term
-  | k :  nat →  term → term
-  | c : term → term
-  | impl : term → term → term
-  | and : term → term → term  
-  | or : term → term → term.
+Inductive Term : Set :=
+  | bottom : Term
+  | var : nat → Term
+  | e : Term → Term
+  | k :  nat →  Term → Term
+  | c : Term → Term
+  | impl : Term → Term → Term
+  | and : Term → Term → Term  
+  | or : Term → Term → Term.
 
 
 (* 
-  Helper definition for sets of terms.
+  Helper definition for sets of Terms.
 *)
-Definition Forms := Ensemble term.
+Definition Forms := Ensemble Term.
 
-Definition Si (t : term) : Forms := Singleton term t.
-Definition In_si (t : term) : In term (Si t) t := In_singleton term t.
-Definition EmptyE : Ensemble term := Empty_set term.
-Definition Ut (u : Forms) (v : Forms) : Forms := Union term u v.
-Definition Compt (x : Forms) (f : term -> term) : Forms :=
-  apply_func term term f x.
+Definition Si (t : Term) : Forms := Singleton Term t.
+Definition In_si (t : Term) : In Term (Si t) t := In_singleton Term t.
+Definition EmptyE : Ensemble Term := Empty_set Term.
+Definition Ut (u : Forms) (v : Forms) : Forms := Union Term u v.
+Definition Compt (x : Forms) (f : Term -> Term) : Forms :=
+  apply_func f x.
+Notation "a ∈ X" := (In Term X a) (at level 17).
+Notation "A ∪ B" := (Ut A B) (at level 19, left associativity).
+Notation "⊥" := bottom.
 
-
-
+Reserved Notation "A ?⊃ B" (at level 18).
+Inductive S : Forms -> Term -> Prop :=
+| AxbS :  ∀ Γ a, (a ∈ Γ) → (Γ ?⊃ a)
+| AxiS :  ∀ Γ a, (⊥ ∈ Γ) → (Γ ?⊃ a)
+| EFixS : ∀ i Γ a, (Γ ∪ (Si (e a))) ?⊃ (k i a)
+| CutS :  ∀ Γ a b,  (Γ ?⊃ a) → ((Γ ∪ (Si a)) ?⊃ b) → (Γ ?⊃ b)
+| OrLS :  ∀ Γ a b c,  ((Γ ∪ (Si a))  ?⊃ c) → ((Γ ∪ (Si b))  ?⊃ c) → ((Γ ∪ (Si (or a b)))  ?⊃ c)
+where "A ?⊃ B" := (S A B).
 (*
   The most important definition:   The Phi  ⊃  t 
 *)
-Definition Ent (x : Forms) (y : term) := Prop.
+Definition Ent (x : Forms) (y : Term) := Prop.
 
 
 Notation "A ⊃ B" := (Ent A B)  (at level 0, no associativity).
 Notation "A |_| B" := (Ut A B) (at level 50, left associativity).
 
-Inductive Axb (a : term) (x : Forms) : (x ⊃ a) :=
+Inductive Axb (a : Term) (x : Forms) : ((Ut x (Si ⊥)) ⊃ a) :=
  AxbE : Axb a x.
-Inductive Axi (a : term) (x : Forms) : ((Ut x (Si a)) ⊃ a) :=
+Inductive Axi (a : Term) (x : Forms) : ((Ut x (Si a)) ⊃ a) :=
  AxiE : Axi a x.
-Inductive EFix (i : nat) (a : term) (x : Forms) : (Ut x (Si (e a))) ⊃ (k i a) :=
+Inductive EFix (i : nat) (a : Term) (x : Forms) : (Ut x (Si (e a))) ⊃ (k i a) :=
 EFixE : EFix i a x.
-Inductive EFixR (i : nat) (a : term) (x : Forms) (v : (x ⊃ (e a))) :
+Inductive EFixR (i : nat) (a : Term) (x : Forms) (v : (x ⊃ (e a))) :
   (x ⊃ (k i a)) :=
-EFixRE : EFixR i a x v.
-Inductive EFixL (i : nat) (a b : term) (x : Forms) (v : (Ut x (Si (e a))) ⊃ b) :
+EFixRE : EFixR i v.
+Inductive EFixL (i : nat) (a b : Term) (x : Forms) (v : (Ut x (Si (e a))) ⊃ b) :
   ((Ut x (Si (k i a))) ⊃ b) :=
-EFixLE : EFixL i a b x v.
+EFixLE : EFixL i v.
 
-Inductive Cut (a b : term) (x : Forms) (u : (x ⊃ a)) (v : ((Ut x (Si a)) ⊃ b)) :
+Inductive Cutt (a b : Term) (x : Forms) (u : (x ⊃ a)) (v : ((Ut x (Si a)) ⊃ b)) :
    (x ⊃ b) :=
-CutE : Cut a b x u v.
+CutE : Cutt u v.
 
-Inductive OrL (a b c : term) (x : Forms) 
+Inductive OrL (a b c : Term) (x : Forms) 
   (u : (Ut x (Si a))  ⊃ c)  
   (v : (Ut x (Si b))  ⊃ c) : ((Ut x (Si (or a b)))  ⊃ c) :=
-OrLE : OrL a b c x u v.
+OrLE : OrL u v.
 
 
-Inductive OrR1 (a b : term) (x : Forms) (u : (x ⊃ a)) : x ⊃ (or a b) :=
-OrR1E : OrR1 a b x u.
+Inductive OrR1 (a b : Term) (x : Forms) (u : (x ⊃ a)) : x ⊃ (or a b) :=
+OrR1E : OrR1 b u.
 
-Lemma triv : forall (a : term), (Si a) ⊃ a.
+Lemma triv : forall (a : Term), (Si a) ⊃ a.
 intros.
 exact (Axi a (Si a) ).
 Defined.
-Inductive OrR2 (a b : term) (x : Forms) (u : (x ⊃ a)) : x ⊃ (or b a) :=
-OrR2E : OrR2 a b x u.
+Inductive OrR2 (a b : Term) (x : Forms) (u : (x ⊃ a)) : x ⊃ (or b a) :=
+OrR2E : OrR2 b u.
 
 
 
-Inductive AndL (a b c : term) (x : Forms) (u : (Ut (Ut x (Si a)) (Si b))  ⊃ c) : 
+Inductive AndL (a b c : Term) (x : Forms) (u : (Ut (Ut x (Si a)) (Si b))  ⊃ c) : 
   (Ut x (Si (and a b)))  ⊃ c :=
-AndLE : AndL a b c x u.
+AndLE : AndL u.
 
 
-Lemma triv_orl2 : forall (a b : term), (Si a) ⊃ (or a b).
+Lemma triv_orl2 : forall (a b : Term), (Si a) ⊃ (or a b).
 intros.
 apply OrR1.
 apply triv.
 Defined.
 
-Lemma xx : forall (a b c : term), 
+Lemma xx : forall (a b c : Term), 
   ((Ut (Si a) (Si b)) ⊃ c)
   -> ((Si (and a b)) ⊃ c).
 intros.
 apply (AndL a b c0 (EmptyE) X).
 Defined.
 
-Inductive AndR (a b : term) (x : Forms) 
+Inductive AndR (a b : Term) (x : Forms) 
   (u : (x ⊃ a)) (v : (x ⊃ b)) : 
     (x ⊃ (and a b)) :=
 AndRE : AndR a b x u v.
 
 
-Inductive ImplL (a b c : term) (x : Forms) 
+Inductive ImplL (a b c : Term) (x : Forms) 
   (u : (x ⊃ a)) 
   (v : ((Ut x (Si b)) ⊃ c)) : 
     (Ut x (Si (impl a b))) ⊃ c :=
 ImplLE : ImplL a b c x u v.
 
-Inductive ImplR (a b : term) (x : Forms) (u : (Ut x (Si a)) ⊃ b) : 
+Inductive ImplR (a b : Term) (x : Forms) (u : (Ut x (Si a)) ⊃ b) : 
   (x ⊃ (impl a b)) :=
 ImplRe : ImplR a b x u.
 
@@ -164,21 +174,21 @@ ImplRe : ImplR a b x u.
 ---------------------
 Ki(X),C(Y),Z ⊃ Ki(a)
 *)
-Inductive Ki (i : nat) (a : term) (x y z : Forms) 
+Inductive Ki (i : nat) (a : Term) (x y z : Forms) 
   (u : ((Ut x (Compt y (fun x => c x))) ⊃ a)) :
     (Ut (Ut (Compt x (fun x => k i x))
      (Compt y (fun x => c x))) z) ⊃ (k i a) :=
 KiE : Ki i a x y z u.
 
-Inductive CL (a b : term) (x : Forms) (u : ((Ut x (Si (e a))) ⊃ b )) :
+Inductive CL (a b : Term) (x : Forms) (u : ((Ut x (Si (e a))) ⊃ b )) :
    ((Ut x (Si (c a))) ⊃ b) :=
 ClE : CL a b x u.
 
-Inductive CR (a : term) (x y : Forms) (u : ((Compt x (fun x => c x)) ⊃ (e a))) :
+Inductive CR (a : Term) (x y : Forms) (u : ((Compt x (fun x => c x)) ⊃ (e a))) :
   (Ut (Compt x (fun x => c x)) y) ⊃ (c a) :=
 CLE : CR a x y u.
 
-Inductive Ind (a b : term) (x y : Forms) 
+Inductive Ind (a b : Term) (x y : Forms) 
   (u : ((Ut (Compt x (fun x => c x)) (Si b)) ⊃ (e a)))
   (v : ((Ut (Compt x (fun x => c x)) (Si b)) ⊃ (e b))) :
     ((Ut (Ut (Compt x (fun x => c x)) y) (Si b)) ⊃ (c a)) :=
@@ -192,20 +202,20 @@ intros.
 auto with sets.
 Defined.
 
-Lemma one : forall (a : term), (Si a) ⊃ a.
+Lemma one : forall (a : Term), (Si a) ⊃ a.
 Proof.
 apply triv.
 Defined.
 
-Lemma two : forall (i : nat) (a b : term), 
+Lemma two : forall (i : nat) (a b : Term), 
   (Ut (Si (k i a)) (Si (k i (impl a b)))) ⊃ (k i b).
 Proof.
 intros.
 apply (Ki i b ((Si a) |_| Si (impl a b)) EmptyE EmptyE ).
 unfold Compt.
 rewrite apply_func_empty.
-rewrite (Union_commutative term).
-rewrite (em term).
+rewrite (Union_commutative Term).
+rewrite (em Term).
 apply (ImplL a b b (Si a)).
 apply triv.
 apply (Axi b (Si a |_| Si b)).
@@ -251,7 +261,7 @@ absurd (In A (Empty_set A) x0).
 *)
 
 
-Lemma three : forall (i : nat) (a : term), 
+Lemma three : forall (i : nat) (a : Term), 
   (EmptyE ⊃ a) -> (EmptyE ⊃ (and (k i a) (c a))).
 Proof.
 intros.
@@ -259,7 +269,7 @@ apply (AndR).
 apply (Ki i a EmptyE EmptyE EmptyE).
 unfold Compt.
 rewrite (apply_func_empty).
-rewrite (em term).
+rewrite (em Term).
 assumption.
 exact (Si a).
 apply (CR a EmptyE EmptyE).
@@ -269,17 +279,17 @@ apply ((EFixR i a EmptyE) X).
 exact (Si bottom).
 Defined.
 
-Definition In_ut (a : term) (x : Forms) : In term (Ut x (Si a)) a := 
-  Union_intror term x (Si a) a (In_si a).
+Definition In_ut (a : Term) (x : Forms) : In Term (Ut x (Si a)) a := 
+  Union_intror Term x (Si a) a (In_si a).
 
 
-Lemma four : forall (a : term), (Si (and (e a) (e (c a)))) ⊃ (c a).
+Lemma four : forall (a : Term), (Si (and (e a) (e (c a)))) ⊃ (c a).
 Proof.
 intros.
 Check (AndL).
 apply (AndL (e a) (e (c a)) (c a) EmptyE).
-rewrite (Union_commutative term).
-rewrite (em term).
+rewrite (Union_commutative Term).
+rewrite (em Term).
 apply (CR a (Si (e a)) (Si (e (c a)))).
 unfold Compt.
 
@@ -297,24 +307,24 @@ apply axi.
 unfold Compt.
 *)
 
-Lemma fife : forall (a : term), (Si (c a)) ⊃ (and (e a) (c (e a))).
+Lemma fife : forall (a : Term), (Si (c a)) ⊃ (and (e a) (c (e a))).
 Proof.
 intros.
 apply andr,  (ind (c a) (e a) EmptyE EmptyE).
 apply (cl a (e a) EmptyE).
-rewrite (em term).
+rewrite (em Term).
 apply axi. exact (In_si (e a)).
 unfold Compt.
 rewrite (apply_func_empty ).
-rewrite (em term).
+rewrite (em Term).
 Check ind.
 Check (ind 
 apply (ind a EmptyE (Si (e a))).
-rewrite (em term).
+rewrite (em Term).
 eauto with sets.
 *)
 
-Lemma six : forall (a b : term), 
+Lemma six : forall (a b : Term), 
   ((Si (c a)) ⊃ b) -> ((Si b) ⊃ (and (e a) (e b))).
 Proof.
 intros a b.
